Remove the dangerous SZ.t ~> erased nat coercions
These kick in when we do not want them to (e.g. if the expected type is
erased bool). Just kill them. Things look more predictable now, but this
may just be a first impression. I also changed `erased nat` to `nat` in
many types and ghost functions, which is the right thing to do, and now
it does in fact seem to work.

src/lib/poly/gemm/Kuiper.Poly.GEMM.Util.fst
@@ -84,7 +84,6 @@ fn matmul_tiled_dotprod
   let mut sum : et = zero;
   let mut bk  : sz = 0sz;
 
-
   while (SZ.(!bk <^ shared))
     invariant
       exists* (vbk : SZ.t) sumv.
@@ -97,22 +96,15 @@ fn matmul_tiled_dotprod
     assert (pure (bi  < (rows   * tile) / tile));
     assert (pure (vbk < (shared * tile) / tile));
     // Sigh.... need to reveal and hide. Terrible UX.
-    let tA = Tiling.gpu_matrix_subtile gA tile tile (hide (reveal bi)) (hide (reveal vbk));
-    let tB = Tiling.gpu_matrix_subtile gB tile tile (hide (reveal vbk)) (hide (reveal bj));
-    assert (rewrites_to tA (Tiling.gpu_matrix_subtile gA tile tile (hide (reveal bi)) (hide (reveal vbk))));
-    assert (rewrites_to tB (Tiling.gpu_matrix_subtile gB tile tile (hide (reveal vbk)) (hide (reveal bj))));
+    let tA = Tiling.gpu_matrix_subtile gA (SZ.v tile) (SZ.v tile) (SZ.v bi) (SZ.v vbk);
+    let tB = Tiling.gpu_matrix_subtile gB (SZ.v tile) (SZ.v tile) (SZ.v vbk) (SZ.v bj);
+    assert (rewrites_to tA (Tiling.gpu_matrix_subtile gA (SZ.v tile) (SZ.v tile) (SZ.v bi) (SZ.v vbk)));
+    assert (rewrites_to tB (Tiling.gpu_matrix_subtile gB (SZ.v tile) (SZ.v tile) (SZ.v vbk) (SZ.v bj)));
 
     Tiling.gpu_matrix_extract_tile gA tile tile bi vbk;
     Tiling.gpu_matrix_extract_tile gB tile tile vbk bj;
 
-    let s' = matmul_dotprod
-      #_ #_
-      #tile #tile #tile
-      // #(Tiling.subtile_layout lA tile tile bi vbk)
-      // #(Tiling.subtile_layout lB tile tile vbk bj)
-      // #(Tiling.c_subtile_layout #_ #_ _ #_ _ _ _ _ #_ #_ #_ #_)
-      // #(Tiling.c_subtile_layout #_ #_ _ #_ _ _ _ _ #_ #_ #_ #_)
-      tA tB i j;
+    let s' = matmul_dotprod tA tB i j;
     sum := !sum `add` s';
 
     ambig_trade_elim ();
